isabelle/Implementation.thy
@@ -25,7 +25,7 @@ datatype Message
   | PublishResponse Slot Term
   | ApplyCommit Slot Term
   | CatchUpRequest
-  | CatchUpResponse Slot "Node set" ClusterState
+  | CatchUpResponse Slot Term "Node set" ClusterState
   | Reboot
 
 text \<open>Some prose descriptions of these messages follows, in order to give a bit more of an
@@ -254,13 +254,14 @@ definition handleApplyCommit :: "Slot \<Rightarrow> Term \<Rightarrow> NodeData 
 
 definition handleCatchUpRequest :: "NodeData \<Rightarrow> (NodeData * Message option)"
   where
-    "handleCatchUpRequest nd = (nd, Some (CatchUpResponse (firstUncommittedSlot nd)
+    "handleCatchUpRequest nd = (nd, Some (CatchUpResponse (firstUncommittedSlot nd) (currentTerm nd)
                                               (currentVotingNodes nd) (currentClusterState nd)))"
 
-definition handleCatchUpResponse :: "Slot \<Rightarrow> Node set \<Rightarrow> ClusterState \<Rightarrow> NodeData \<Rightarrow> NodeData"
+definition handleCatchUpResponse :: "Slot \<Rightarrow> Term \<Rightarrow> Node set \<Rightarrow> ClusterState \<Rightarrow> NodeData \<Rightarrow> NodeData"
   where
-    "handleCatchUpResponse i conf cs nd \<equiv>
+    "handleCatchUpResponse i t conf cs nd \<equiv>
       if firstUncommittedSlot nd < i
+        \<and> t = currentTerm nd
         then nd \<lparr> firstUncommittedSlot := i
                 , lastAcceptedValue := NoOp
                 , lastAcceptedTerm := None
@@ -326,8 +327,8 @@ definition ProcessMessage :: "NodeData \<Rightarrow> RoutedMessage \<Rightarrow>
               \<Rightarrow> (handleApplyCommit i t nd, None)
           | CatchUpRequest
               \<Rightarrow> respondToSender (handleCatchUpRequest nd)
-          | CatchUpResponse i conf cs
-              \<Rightarrow> (handleCatchUpResponse i conf cs nd, None)
+          | CatchUpResponse i t conf cs
+              \<Rightarrow> (handleCatchUpResponse i t conf cs nd, None)
           | Reboot
               \<Rightarrow> (handleReboot nd, None)
         else (nd, None)"
